src/lib/kuiper/Kuiper.Array.fsti
@@ -379,3 +379,43 @@ fn gpu_slice_gather_underspec
   ensures
     exists* v.
       gpu_pts_to_slice arr #f m n v
+
+val adjacent
+  (#a : Type u#0)
+  (#s1 #s2 : nat)
+  (arr1 : gpu_array a s1)
+  (arr2 : gpu_array a s2)
+  : slprop
+
+ghost
+fn gpu_array_cut
+  (#a : Type u#0)
+  (#sz : nat)
+  (arr : gpu_array a sz)
+  (#f : perm) // FIXME: if we use 'f, it gets type 'real' instead of 'perm'
+  (k : SZ.t{ k <= sz })
+  (#s : erased (seq a){ Seq.length s == sz })
+  requires
+    gpu_pts_to_array arr #f s
+  returns
+    p : (gpu_array a k & gpu_array a (sz - k))
+  ensures
+    gpu_pts_to_array p._1 #f (seq_take k s) **
+    gpu_pts_to_array p._2 #f (seq_drop k s) **
+    adjacent p._1 p._2
+
+ghost
+fn gpu_array_paste
+  (#a : Type u#0)
+  (#sz1 #sz2 : nat)
+  (arr1 : gpu_array a sz1)
+  (arr2 : gpu_array a sz2)
+  (#f : perm) // FIXME: if we use 'f, it gets type 'real' instead of 'perm'
+  requires
+    gpu_pts_to_array arr1 #f 's1 **
+    gpu_pts_to_array arr2 #f 's2 **
+    adjacent arr1 arr2
+  returns
+    arr : gpu_array a (sz1 + sz2)
+  ensures
+    gpu_pts_to_array arr #f (Seq.append 's1 's2)
